---
tags:
  - atom
  - math
---
#TODO 

This is obvious but it has wide implications.
$$ f(x) = \sum_{n=i}^\infty a_n(x) \implies f(u) = \sum_{n=i}^\infty a_n(u) $$

> [!example]
> $$\begin{array}{c}
> 	\displaystyle e^x = \sum_{n=0}^\infty \dfrac{x^n}{n!} = x + \dfrac{x^2}{2!} + \dfrac{x^3}{3!} + \dfrac{x^4}{4!} + \cdots \\
> 	\Big\Updownarrow \\
> 	\displaystyle e^{2x} = \sum_{n=0}^\infty \dfrac{x^{2n}}{n!} = x^2 + \dfrac{x^4}{2!} + \dfrac{x^6}{3!} + \dfrac{x^8}{4!} + \cdots \\
> \end{array}$$