---
tags:
  - atom
  - math
---

$$
\begin{array}{l c l}
	\sinh^{-1}x = \ln(x + \sqrt{x^2 + 1}) && x \in \R \\
	\cosh^{-1}x = \ln(x + \sqrt{x^2 - 1}) && x \in \left[ 1, \infty \right) \\
	\tanh^{-1}x = \dfrac{1}{2}\ln\left(\dfrac{1+x}{1-x}\right) && x \in \left( -1, 1 \right) \\
\end{array}
$$

$$
\begin{array}{l c l}
	\dfrac{d}{dx} \left( \sinh^{-1} x \right) = \dfrac{1}{\sqrt{1 + x^2}} &&
	\dfrac{d}{dx} \left( \text{csch}^{-1}\:x \right) = -\dfrac{1}{|x|\sqrt{x^2 + 1}}
	\\
	\dfrac{d}{dx} \left( \cosh^{-1} x \right) = \dfrac{1}{\sqrt{x^2 - 1}} &&
	\dfrac{d}{dx} \left( \text{sech}^{-1}\:x \right) = -\dfrac{1}{x\sqrt{1 - x^2}}
	\\
	\dfrac{d}{dx} \left( \tanh^{-1} x \right) = \dfrac{1}{1 - x^2} &&
	\dfrac{d}{dx} \left( \coth^{-1} x \right) = \dfrac{1}{1 - x^2}
\end{array}
$$

\[[[Hyperbolic Functions]], [[Inverse Functions|Inverse Functions]]\]

