---
tags:
  - atom
  - math
  - discrete
---
Suppose $G$ [[Group Actions|acts]] on a [[Sets|set]] $S$.
> [!definition] Orbit of a Point
> The *orbit* of a point $s \in S$ is the [[Sets|set]]
> $$\text{Orb}(s) = \{ g(s) : g \in G \}$$
> *the points reachable from $s$.*

> [!definition] Orbits of a Action
> The *orbits* of an [[Group Actions|action]] is an [[Equivalence Classes|equivalence class]].
> $$ [s] = \text{Orb}(s) $$
> *a [[Partitions|part]] in the [[Partitions|partition]] generated by $\mathit{Orb(s)}$.*

> [!definition] Stabilizer
> The *stabilizer* of a point $s \in S$ is the [[Subgroups|subgroup]]
> $$\text{Stab}(s) = \{ g \in G : g(s) = s \}$$
> *the [[Groups|group]] elements that don't affect $\mathit{s}$.*

> [!definition]- Fixed Set
> The *fixed* [[Sets|set]] of $g \in G$ is the [[Subsets|subset]]
> $$\text{Fix}(g) = \{ s \in S : g(s) = s \}$$
> *the points unaffected by the given [[Groups|group]] element.*

# Lemmas
> [!lemma]- Suppose $G$ is a [[Groups|group]] acting on a [[Sets|set]] $S$. For $s \in S$, $\text{Stab}(s)$ is a [[Subgroups|subgroup]] of $G$.
> Let $g,h \in\text{Stab}(s)$. By the [[Subgroups|one-step subgroup test]], $\text{Stab}(s)$ is a [[Subgroups|subgroup]] iff $gh^{-1} \in \text{Stab}(s)$.
> 
> By the definition of [[Group Actions|group action]],
> $$gh(s) = g(h(s)).$$
> Since $h \in\text{Stab}(s)$, $h(s) = s$, so $h^{-1}(s) = s$.
> $$\hspace{1em}\begin{align}
> 	h^{-1}(s) &= h(s) \\
> 	g(h^{-1}(s)) &= g(h(s)) \\
> 	gh^{-1}(s) &= g(s) \\
> 	&= g(s). \\
> \end{align}$$
> Similarly, since $g \in\text{Stab}(s)$, $g(s) = s$, so
> $$gh^{-1}(s) = s,$$
> thus, $gh^{-1} \in\text{Stab}(s)$.

> [!lemma]- Suppose $G$ is a [[Groups|group]] acting on a [[Sets|set]] $S$. For $s \in S$ and $g,h \in G$, $g(s) = h(s)$ iff $g$ and $h$ lie in the same [[Cosets|coset]] of $\text{Stab}(s)$;$$g(s) = h(s) \iff \exists c \in G : g,h \in c \, \text{Stab}(s)$$
> $(\impliedby)$
> Suppose $g,h$ lie in the same [[Cosets|coset]] of $\text{Stab}(s)$.
> 
> By the definition of a *stabilizer*, $g \in g\,\text{Stab}(s)$ and $h \in h\,\text{Stab}(s)$ (take $e \in\text{Stab}(s)$). Thus, the premise gives
> $$g\,\text{Stab}(s) = h\,\text{Stab}(s).$$
> Since $g \in g\,\text{Stab(s)}$, $g \in h\,\text{Stab}(s)$, meaning $g = hf$ for some $f \in\text{Stab}(s)$. Then
> $$\begin{align}
> 	g(s) &= hf(s) \\
> 	&= h(f(s)) \\
> 	&= h(s) && f \in \text{Stab(s)} \\
> \end{align}$$
> 
> $\left( \implies \right)$
> Suppose $g(s) = h(s)$. 
> $$g(s) = h(s) \implies g^{-1}h(s) = s \implies g^{-1}h \in \text{Stab}(s).$$
> Let $f = g^{-1}h$. 
> 
> Then $h = gf$, meaning $h \in g\,\text{Stab}(s)$, as $f \in\text{Stab}(s)$.
> 
> Similarly, $g = ge$, meaning $g \in g\,\text{Stab}(s)$, as $e \in\text{Stab(s)}$.
> 
> Thus, $g$ (and thus $h$) satisfy the conditions for $c$.